src/program_proof/chat/kt/kt.v
@@ -5,6 +5,479 @@ From Goose.github_com.mit_pdos.secure_chat Require Import kt.
 From Perennial.program_proof.chat.kt Require Import shared shim.
 From iris.unstable.base_logic Require Import mono_list.
 
-Section clerk.
+Section common.
+Context `{!heapGS Σ, !mono_listG UnameKey.t Σ}.
+
+Lemma wp_injestNewLog ptr_currLog currLog sl_newLogB newLogB :
+  {{{
+    "HcurrLog" ∷ KeyLog.own ptr_currLog currLog ∗
+    "HnewLogB" ∷ own_slice_small sl_newLogB byteT 1 newLogB
+  }}}
+  injestNewLog #ptr_currLog (slice_val sl_newLogB)
+  {{{
+    ptr_newLog newLog (err:u64), RET (#ptr_newLog, #err);
+    "HcurrLog" ∷ KeyLog.own ptr_currLog currLog ∗
+    "HnewLog" ∷ KeyLog.own ptr_newLog newLog ∗
+    if bool_decide (#err = #0) then
+      "%Henc" ∷ ⌜KeyLog.encodes newLogB newLog⌝ ∗
+      "%Hprefix" ∷ ⌜currLog.(KeyLog.Log) `prefix_of` newLog.(KeyLog.Log)⌝
+    else True%I
+  }}}.
+Proof. Admitted.
+
+Definition lb_pred γ (log:KeyLog.t) : iProp Σ :=
+  "Hlb_log" ∷ mono_list_lb_own γ log.(KeyLog.Log).
+
+(* I think this implicitly assumes that for a particular list u8,
+   there's only one log that could encode to it. *)
+Definition lb_sig_pred γ : (list u8 → iProp Σ) :=
+  λ logB, (∃ log, ⌜KeyLog.encodes logB log⌝ ∗ lb_pred γ log)%I.
+
+End common.
+
+Section keyServ.
 Context `{!heapGS Σ}.
-End clerk.
+
+Lemma wp_keyServ_new :
+  {{{ True }}}
+  newKeyServ #()
+  {{{ ptr_keyServ, RET #ptr_keyServ; True }}}.
+Proof. Admitted.
+
+Lemma wp_keyServ_start l (addr:u64) :
+  {{{ True }}}
+  keyServ__start #l #addr
+  {{{ RET #(); True }}}.
+Proof. Admitted.
+
+End keyServ.
+
+Section auditor.
+Context `{!heapGS Σ, !mono_listG UnameKey.t Σ}.
+
+Record adtrParam :=
+  AdtrParam {
+    γ : gname;
+    Hon : bool
+  }.
+
+Definition lockR_adtr l param log : iProp Σ :=
+  ∃ ptr_log sk,
+  "Hlog" ∷ KeyLog.own ptr_log log ∗
+  "Hauth_log" ∷ mono_list_auth_own param.(γ) 1 log.(KeyLog.Log) ∗
+  "Hptr_log" ∷ l ↦[auditor :: "log"] #ptr_log ∗
+  "Hsk" ∷ own_sk sk (lb_sig_pred param.(γ)) param.(Hon) ∗
+  "Hptr_sk" ∷ l ↦[auditor :: "key"] #sk.
+
+Definition is_adtr l param log : iProp Σ :=
+  ∃ lk,
+  "#HlkR" ∷ is_lock nroot #lk (lockR_adtr l param log) ∗
+  "#Hlk" ∷ readonly (l ↦[auditor :: "mu"] #lk).
+
+Lemma wp_auditor_new param sk :
+  {{{
+    "Hsk" ∷ own_sk sk (lb_sig_pred param.(γ)) param.(Hon) ∗
+    "Hauth_log" ∷ mono_list_auth_own param.(γ) 1 []
+  }}}
+  newAuditor #sk
+  {{{
+    ptr_adtr, RET #ptr_adtr;
+    "#Hadtr" ∷ is_adtr ptr_adtr param (KeyLog.mk [])
+  }}}.
+Proof. Admitted.
+
+(* TODO: proving this will actually require proving true/true on all
+   the handler funcs, but I'll save that for later. *)
+Lemma wp_auditor_start l param log (addr:u64) :
+  {{{
+    "#Hadtr" ∷ is_adtr l param log
+  }}}
+  auditor__start #l #addr
+  {{{ RET #(); True }}}.
+Proof. Admitted.
+End auditor.
+
+Section keycli.
+Context `{!heapGS Σ, !mono_listG UnameKey.t Σ}.
+
+Definition own_keyCli l log adtrParams : iProp Σ :=
+  ∃ ptr_log ptr_serv_rpc adtrs sl_adtrs vks sl_vks,
+  "Hlog" ∷ KeyLog.own ptr_log log ∗
+  "Hptr_log" ∷ l ↦[keyCli :: "log"] #ptr_log ∗
+  "Hserv" ∷ own_rpc_cli ptr_serv_rpc ∗
+  "Hptr_serv" ∷ l ↦[keyCli :: "serv"] #ptr_serv_rpc ∗
+  "Hadtrs" ∷ ([∗ list] ptr_adtr ∈ adtrs, own_rpc_cli ptr_adtr) ∗
+  "Hsl_adtrs" ∷ own_slice_small sl_adtrs ptrT 1 adtrs ∗
+  "Hptr_adtrs" ∷ l ↦[keyCli :: "adtrs"] (slice_val sl_adtrs) ∗
+  "#Hvks" ∷ ([∗ list] vk;param ∈ vks;adtrParams,
+    is_vk vk (lb_sig_pred param.(γ)) param.(Hon)) ∗
+  "Hsl_vks" ∷ own_slice_small sl_vks ptrT 1 vks ∗
+  "Hptr_vks" ∷ l ↦[keyCli :: "adtrKeys"] (slice_val sl_vks).
+
+Lemma wp_keyCli_new (serv:u64) sl_adtrAddrs (adtrAddrs:list u64) sl_vks vks adtrParams q1 q2 :
+  {{{
+    "HadtrAddrs" ∷ own_slice_small sl_adtrAddrs uint64T q1 adtrAddrs ∗
+    "#Hvks" ∷ ([∗ list] vk;param ∈ vks;adtrParams,
+      is_vk vk (lb_sig_pred param.(γ)) param.(Hon)) ∗
+    "Hsl_vks" ∷ own_slice_small sl_vks ptrT q2 vks
+  }}}
+  newKeyCli #serv (slice_val sl_adtrAddrs) (slice_val sl_vks)
+  {{{
+    ptr_keyCli, RET #ptr_keyCli;
+    "HadtrAddrs" ∷ own_slice_small sl_adtrAddrs uint64T q1 adtrAddrs ∗
+    "HkeyCli" ∷ own_keyCli ptr_keyCli (KeyLog.mk []) adtrParams
+  }}}.
+Proof. Admitted.
+
+Lemma wp_keyCli_reg ptr_keyCli ptr_entry entry log adtrParams :
+  {{{
+    "HkeyCli" ∷ own_keyCli ptr_keyCli log adtrParams ∗
+    "Hentry" ∷ UnameKey.own ptr_entry entry
+  }}}
+  keyCli__register #ptr_keyCli #ptr_entry
+  {{{
+    (epoch err:u64) newLog, RET (#epoch, #err);
+    "HkeyCli" ∷ own_keyCli ptr_keyCli newLog adtrParams ∗
+    "Hentry" ∷ UnameKey.own ptr_entry entry ∗
+    if bool_decide (#err = #0) then
+      "%Hprefix" ∷ ⌜log.(KeyLog.Log) `prefix_of` newLog.(KeyLog.Log)⌝ ∗
+      "%Helem_of" ∷ ⌜newLog.(KeyLog.Log) !! int.nat epoch = Some entry⌝
+    else True%I
+  }}}.
+Proof. Admitted.
+
+Lemma wp_keyCli_look ptr_keyCli (uname:u64) log adtrParams :
+  {{{
+    "HkeyCli" ∷ own_keyCli ptr_keyCli log adtrParams
+  }}}
+  keyCli__lookup #ptr_keyCli #uname
+  {{{
+    (epoch:u64) sl_key (key:list u8) (err:u64) newLog,
+    RET (#epoch, slice_val sl_key, #err);
+    "HkeyCli" ∷ own_keyCli ptr_keyCli newLog adtrParams ∗
+    if bool_decide (#err = #0) then
+      "Hkey" ∷ own_slice_small sl_key byteT 1 key ∗
+      "%Hprefix" ∷ ⌜log.(KeyLog.Log) `prefix_of` newLog.(KeyLog.Log)⌝ ∗
+      "%Helem_of" ∷ ⌜newLog.(KeyLog.Log) !! int.nat epoch = Some (UnameKey.mk uname key)⌝
+    else True%I
+  }}}.
+Proof. Admitted.
+
+Lemma wp_keyCli_audit ptr_keyCli (adtrId:u64) log adtrParams :
+  {{{
+    "HkeyCli" ∷ own_keyCli ptr_keyCli log adtrParams ∗
+    "%HadtrId" ∷ ⌜int.nat adtrId < length adtrParams⌝
+  }}}
+  keyCli__audit #ptr_keyCli #adtrId
+  {{{
+    (epoch err:u64) param, RET (#epoch, #err);
+    "HkeyCli" ∷ own_keyCli ptr_keyCli log adtrParams ∗
+    "%Hparam" ∷ ⌜adtrParams !! int.nat adtrId = Some param⌝ ∗
+    if bool_decide (#err = #0) && param.(Hon) then
+      (* take is 1-idx'd, epoch is 0-idx'd. *)
+      "#Hlb_log" ∷ mono_list_lb_own param.(γ) (take (int.nat epoch + 1) log.(KeyLog.Log))
+    else True%I
+  }}}.
+Proof. Admitted.
+
+End keycli.
+
+Section tests.
+Context `{!heapGS Σ, !mono_listG UnameKey.t Σ}.
+
+Lemma wp_testAuditPass (servAddr:u64) sl_adtrAddrs (addr0 addr1 addr2:u64) :
+  {{{
+    "HadtrAddrs" ∷ own_slice_small sl_adtrAddrs uint64T 1 [addr0; addr1; addr2]
+  }}}
+  testAuditPass #servAddr (slice_val sl_adtrAddrs)
+  {{{ RET #(); True }}}.
+Proof using heapGS0 mono_listG0 Σ.
+  iIntros (Φ) "H HΦ"; iNamed "H".
+  rewrite /testAuditPass.
+
+  (* Start key server. *)
+  wp_apply wp_fork.
+  {
+    wp_apply wp_keyServ_new.
+    iIntros (?) "_".
+    by wp_apply wp_keyServ_start.
+  }
+  wp_apply wp_Sleep.
+
+  (* Make auditor keys. *)
+  iMod (mono_list_own_alloc []) as (γ0) "(Hauth0 & _)".
+  iMod (mono_list_own_alloc []) as (γ1) "(Hauth1 & _)".
+  iMod (mono_list_own_alloc []) as (γ2) "(Hauth2 & _)".
+  wp_apply (wp_MakeKeys (lb_sig_pred γ0) false).
+  { iPureIntro. apply _. }
+  iIntros (badSk0 badVk0) "H"; iNamed "H";
+    iRename "Hsk" into "HbadSk0"; iRename "Hvk" into "HbadVk0".
+  wp_apply (wp_MakeKeys (lb_sig_pred γ1) true).
+  { iPureIntro. apply _. }
+  iIntros (goodSk0 goodVk0) "H"; iNamed "H";
+    iRename "Hsk" into "HgoodSk0"; iRename "Hvk" into "HgoodVk0".
+  wp_apply (wp_MakeKeys (lb_sig_pred γ2) false).
+  { iPureIntro. apply _. }
+  iIntros (badSk1 badVk1) "H"; iNamed "H";
+    iRename "Hsk" into "HbadSk1"; iRename "Hvk" into "HbadVk1".
+
+  wp_apply wp_ref_of_zero; [done|].
+  iIntros (ptr_adtrVks) "Hptr_adtrVks".
+  wp_load.
+  wp_apply wp_SliceAppend_to_zero; [done|].
+  iIntros (adtrVks') "HadtrVks'".
+  wp_store.
+  wp_load.
+  wp_apply (wp_SliceAppend with "[$]").
+  iIntros (adtrVks'') "HadtrVks''".
+  wp_store.
+  wp_load.
+  wp_apply (wp_SliceAppend with "[$]").
+  iIntros (adtrVks) "HadtrVks".
+  wp_store.
+  iDestruct (own_slice_to_small with "HadtrVks") as "HadtrVks".
+  iSimpl in "HadtrVks".
+  clear adtrVks' adtrVks''.
+
+  (* Start auditors. *)
+  iDestruct "HadtrAddrs" as "[HadtrAddrs3 [Haddrs0 [Haddrs1 Haddrs2]]]".
+  pose (AdtrParam γ0 false) as param0.
+  wp_apply (wp_fork with "[Hauth0 HbadSk0 Haddrs0]").
+  {
+    iIntros "!>".
+    wp_apply (wp_auditor_new param0 with "[$]").
+    iIntros (?) "H"; iNamed "H".
+    wp_apply (wp_SliceGet with "[$Haddrs0]"); [done|].
+    iIntros "_".
+    by wp_apply (wp_auditor_start with "[$]").
+  }
+  pose (AdtrParam γ1 true) as param1.
+  wp_apply (wp_fork with "[Hauth1 HgoodSk0 Haddrs1]").
+  {
+    iIntros "!>".
+    wp_apply (wp_auditor_new param1 with "[$]").
+    iIntros (?) "H"; iNamed "H".
+    wp_apply (wp_SliceGet with "[$Haddrs1]"); [done|].
+    iIntros "_".
+    by wp_apply (wp_auditor_start with "[$]").
+  }
+  pose (AdtrParam γ2 false) as param2.
+  wp_apply (wp_fork with "[Hauth2 HbadSk1 Haddrs2]").
+  {
+    iIntros "!>".
+    wp_apply (wp_auditor_new param2 with "[$]").
+    iIntros (?) "H"; iNamed "H".
+    wp_apply (wp_SliceGet with "[$Haddrs2]"); [done|].
+    iIntros "_".
+    by wp_apply (wp_auditor_start with "[$]").
+  }
+  wp_apply wp_Sleep.
+
+  (* Make keyCli's. *)
+  remember ([badVk0; goodVk0; badVk1]) as vks.
+  remember ([param0; param1; param2]) as params.
+  iAssert ([∗ list] vk ; p ∈ vks ; params,
+    is_vk vk (lb_sig_pred p.(kt.γ)) p.(kt.Hon))%I
+    as "#His_vks"; [naive_solver|].
+  iClear "HbadVk0 HgoodVk0 HbadVk1".
+  iDestruct "HadtrVks" as "[HadtrVks0 [HadtrVks1 HadtrVks2]]".
+  wp_load.
+  wp_apply (wp_keyCli_new with "[$]").
+  iIntros (cReg) "H"; iNamed "H"; iRename "HkeyCli" into "HcReg".
+  wp_load.
+  wp_apply (wp_keyCli_new with "[$]").
+  iIntros (cLook0) "H"; iNamed "H"; iRename "HkeyCli" into "HcLook0".
+  wp_load.
+  wp_apply (wp_keyCli_new with "[$]").
+  iIntros (cLook1) "H"; iNamed "H"; iRename "HkeyCli" into "HcLook1".
+
+  (* Register a key. *)
+  wp_apply wp_StringToBytes.
+  iIntros (key0) "Hkey0".
+  iDestruct (own_slice_to_small with "Hkey0") as "Hkey0".
+  wp_apply wp_allocStruct; [val_ty|].
+  iIntros (goodEntry) "HgoodEntry".
+  iDestruct (struct_fields_split with "HgoodEntry") as "H".
+  iNamed "H".
+  wp_apply (wp_keyCli_reg with "[$HcReg Uname Key Hkey0]").
+  {
+    instantiate (1:=UnameKey.mk _ _).
+    (* Note: iFrame could handle this without the rewrite, but it performs some weird
+       unfolding that makes the context after the wp_apply verbose. *)
+    rewrite /UnameKey.own /=.
+    iFrame.
+  }
+  iIntros (epoch err0 newLog0) "H"; iNamed "H";
+    iRename "HkeyCli" into "HcReg";
+    iRename "Hentry" into "HgoodEntry".
+  wp_apply wp_Assume.
+  iIntros "_"; iClear (epoch err0) "H".
+
+  (* Lookup that uname. *)
+  wp_apply (wp_keyCli_look with "[$HcLook0]").
+  iIntros (epoch0 sl_retKey0 retKey0 err1 newLog1) "H"; iNamed "H";
+    iRename "HkeyCli" into "HcLook0".
+  wp_apply wp_Assume.
+  iIntros "%Herr".
+  apply bool_decide_eq_true in Herr.
+  rewrite Herr.
+  iSimpl in "H".
+  iNamed "H"; iRename "Hkey" into "HretKey0";
+    move: {Herr err1 Hprefix} Helem_of => Helem_of1.
+
+  wp_apply (wp_keyCli_look with "[$HcLook1]").
+  iIntros (epoch1 sl_retKey1 retKey1 err2 newLog2) "H"; iNamed "H";
+    iRename "HkeyCli" into "HcLook1".
+  wp_apply wp_Assume.
+  iIntros "%Herr".
+  apply bool_decide_eq_true in Herr.
+  rewrite Herr.
+  iSimpl in "H".
+  iNamed "H"; iRename "Hkey" into "HretKey1";
+    move: {Herr err2 Hprefix} Helem_of => Helem_of2.
+
+  (* Start auditor RPC clients. *)
+  wp_apply (wp_SliceGet with "[$HadtrAddrs]"); [done|].
+  iIntros "HadtrAddrs".
+  wp_apply wp_rpc_MakeClient.
+  iIntros (badAdtr0) "H"; iNamed "H"; iRename "Hurpc" into "HbadAdtr0".
+  wp_apply (wp_SliceGet with "[$HadtrAddrs]"); [done|].
+  iIntros "HadtrAddrs".
+  wp_apply wp_rpc_MakeClient.
+  iIntros (goodAdtr0) "H"; iNamed "H"; iRename "Hurpc" into "HgoodAdtr0".
+  wp_apply (wp_SliceGet with "[$HadtrAddrs]"); [done|].
+  iIntros "HadtrAddrs".
+  wp_apply wp_rpc_MakeClient.
+  iIntros (badAdtr1) "H"; iNamed "H"; iRename "Hurpc" into "HbadAdtr1".
+
+  (* Update bad auditors with bad log. *)
+  wp_apply wp_StringToBytes.
+  iIntros (key1) "Hkey1".
+  iDestruct (own_slice_to_small with "Hkey1") as "Hkey1".
+  wp_apply wp_allocStruct; [val_ty|].
+  iIntros (badEntry) "HbadEntry".
+  iDestruct (struct_fields_split with "HbadEntry") as "H".
+  iNamed "H".
+  wp_apply KeyLog.wp_New.
+  iIntros (ptr_badLog) "HbadLog".
+  wp_apply (KeyLog.wp_Append with "[$HbadLog Uname Key Hkey1]").
+  {
+    instantiate (1:=UnameKey.mk _ _).
+    rewrite /UnameKey.own /=.
+    iFrame.
+  }
+  iIntros "H"; iNamed "H"; iRename "Harg" into "HbadLog".
+  wp_apply (KeyLog.wp_Encode with "[$HbadLog]").
+  iIntros (sl_badLogB badLogB) "H"; iNamed "H";
+    iClear (badEntry ptr_badLog Henc key1) "Harg";
+    iRename "HargB" into "HbadLogB".
+  wp_apply wp_NewSlice.
+  iIntros (emptyB) "_".
+  wp_apply (wp_rpc_Call with "[$HbadAdtr0 $HbadLogB]").
+  iIntros (err3 out) "H"; iNamed "H";
+    iRename "Hrpc" into "HbadAdtr0";
+    iRename "Hin" into "HbadLogB".
+  wp_apply wp_Assume.
+  iIntros "_"; iClear (err3 out) "H".
+  wp_apply (wp_rpc_Call with "[$HbadAdtr1 $HbadLogB]").
+  iIntros (err4 out) "H"; iNamed "H";
+    iRename "Hrpc" into "HbadAdtr1".
+  wp_apply wp_Assume.
+  iIntros "_";
+    iClear (err4 out sl_badLogB badLogB) "H Hin".
+
+  (* Update good auditor with good log. *)
+  wp_apply KeyLog.wp_New.
+  iIntros (ptr_goodLog) "HgoodLog".
+  wp_apply (KeyLog.wp_Append with "[$HgoodLog $HgoodEntry]").
+  iIntros "H"; iNamed "H"; iRename "Harg" into "HgoodLog".
+  wp_apply (KeyLog.wp_Encode with "[$HgoodLog]").
+  iIntros (sl_goodLogB goodLogB) "H"; iNamed "H";
+    iClear (goodEntry ptr_goodLog Henc) "Harg";
+    iRename "HargB" into "HgoodLogB".
+  wp_apply (wp_rpc_Call with "[$HgoodAdtr0 $HgoodLogB]").
+  iIntros (err5 out) "H"; iNamed "H";
+    iRename "Hrpc" into "HgoodAdtr0".
+  wp_apply wp_Assume.
+  iIntros "_";
+    iClear (err5 out sl_goodLogB goodLogB emptyB) "H Hin".
+
+  (* Run keyCli audits. *)
+  wp_apply (wp_keyCli_audit with "[$HcLook0]"); [naive_solver|].
+  iIntros (epoch err param) "H"; iNamed "H";
+    iRename "HkeyCli" into "HcLook0";
+    wp_pures;
+    iClear (epoch err param Hparam) "H".
+  wp_apply (wp_keyCli_audit with "[$HcLook0]"); [naive_solver|].
+  iIntros (auditEpoch0 err6 param) "H"; iNamed "H";
+    iRename "HkeyCli" into "HcLook0".
+  wp_apply wp_Assume.
+  iIntros "%Herr".
+  apply bool_decide_eq_true in Herr.
+  rewrite Herr.
+  assert (int.nat 1%Z = 1) as H by word;
+    rewrite H in Hparam;
+    clear H.
+  assert (param = param1) by naive_solver;
+    subst param.
+  iSimpl in "H"; iNamed "H";
+    iRename "Hlb_log" into "Hlb_cLook0";
+    clear err6 Herr Hparam.
+
+  wp_apply (wp_keyCli_audit with "[$HcLook1]"); [naive_solver|].
+  iIntros (epoch err param) "H"; iNamed "H";
+    iRename "HkeyCli" into "HcLook1";
+    wp_pures;
+    iClear (epoch err param Hparam) "H".
+  wp_apply (wp_keyCli_audit with "[$HcLook1]"); [naive_solver|].
+  iIntros (auditEpoch1 err7 param) "H"; iNamed "H";
+    iRename "HkeyCli" into "HcLook1".
+  wp_apply wp_Assume.
+  iIntros "%Herr".
+  apply bool_decide_eq_true in Herr.
+  rewrite Herr.
+  assert (int.nat 1%Z = 1) as H by word;
+    rewrite H in Hparam;
+    clear H.
+  assert (param = param1) by naive_solver;
+    subst param.
+  iSimpl in "H"; iNamed "H";
+    iRename "Hlb_log" into "Hlb_cLook1";
+    clear err7 Herr Hparam.
+
+  (* Final assert. *)
+  wp_apply (wp_and2 _ _ _ _ True%I); [by wp_pures..|].
+  wp_if_destruct; move: Heqb => HifEq.
+  2: by iApply "HΦ".
+  move: HifEq => [HepochEq [Hepoch0Leq Hepoch1Leq]].
+  wp_apply (wp_BytesEqual with "[$HretKey0 $HretKey1]").
+  iIntros (keysEqb) "H"; iNamed "H";
+    iRename "Hb0" into "HretKey0";
+    iRename "Hb1" into "HretKey1";
+    move: Heqb => HkeysEqb.
+  (* Hard to touch the (take list) inside Hlb since we don't know
+     the log len. Instead, try to reason about the lookup. *)
+  iDestruct (mono_list_idx_own_get with "[$Hlb_cLook0]") as "Hidx0".
+  {
+    (* When we take some number of elements, if we take more
+       than our lookup index, that reduces to a normal lookup. *)
+    assert (int.nat epoch0 < int.nat auditEpoch0 + 1) as H by word.
+    rewrite lookup_take; [apply Helem_of1|apply H].
+  }
+  iDestruct (mono_list_idx_own_get with "[$Hlb_cLook1]") as "Hidx1".
+  {
+    assert (int.nat epoch1 < int.nat auditEpoch1 + 1) as H by word.
+    rewrite lookup_take; [apply Helem_of2|apply H].
+  }
+  (* TODO: not sure why word doesn't handle this. *)
+  assert (epoch0 = epoch1) as H by naive_solver;
+    iEval (rewrite H) in "Hidx0";
+    clear H.
+  iDestruct (mono_list_idx_agree with "Hidx0 Hidx1") as "%HkeysEq".
+  wp_apply wp_Assert.
+  1: destruct keysEqb; [done|naive_solver].
+  wp_pures.
+  by iApply "HΦ".
+Qed.
+
+End tests.
